Evaluation rules

FOmegaC/LemmasTyping.v
@@ -464,27 +464,27 @@ Qed.
 Hint Resolve tm_sub : ws.
 
 
-Record WtRed (Γ Δ: Env) (ζγd ζγe ζ1 ζ2: Sub Exp) : Prop :=
-  { wtd_tyvar : ∀ {α k},
+Record WtCoSub (Γ Δ: Env) (ζγ ζγi ζ1 ζ2: Sub Exp) : Prop :=
+  { wcs_tyvar : ∀ {α k},
                   ⟨ α ∷ k ∈ Γ ⟩ →
-                  ⟨ Δ ⊢ ζγd α : ζ1 α ~ ζ2 α ∷ k ⟩;
-    wtd_covar : ∀ {c τ1 τ2 k},
+                  ⟨ Δ ⊢ ζγ α : ζ1 α ~ ζ2 α ∷ k ⟩;
+    wcs_covar : ∀ {c τ1 τ2 k},
                   ⟨ c : τ1 ~ τ2 ∷ k ∈ Γ ⟩ →
-                  ⟨ Δ ⊢ ζγd c : τ1[ζ1] ~ τ2[ζ2] ∷ k ⟩;
-    wte_tyvar : ∀ {α k},
+                  ⟨ Δ ⊢ ζγ c : τ1[ζ1] ~ τ2[ζ2] ∷ k ⟩;
+    wcs_tyvari : ∀ {α k},
                   ⟨ α ∷ k ∈ Γ ⟩ →
-                  ⟨ Δ ⊢ ζγe α : ζ2 α ~ ζ1 α ∷ k ⟩;
-    wte_covar : ∀ {c τ1 τ2 k},
+                  ⟨ Δ ⊢ ζγi α : ζ2 α ~ ζ1 α ∷ k ⟩;
+    wcs_covari : ∀ {c τ1 τ2 k},
                   ⟨ c : τ1 ~ τ2 ∷ k ∈ Γ ⟩ →
-                  ⟨ Δ ⊢ ζγe c : τ1[ζ2] ~ τ2[ζ1] ∷ k ⟩;
+                  ⟨ Δ ⊢ ζγi c : τ1[ζ2] ~ τ2[ζ1] ∷ k ⟩;
     wtsub_left :> ⟨ ζ1 : Γ => Δ ⟩;
     wtsub_right :> ⟨ ζ2 : Γ => Δ ⟩;
   }.
 
-Hint Resolve wtd_tyvar : ws.
-Hint Resolve wtd_covar : ws.
-Hint Resolve wte_tyvar : ws.
-Hint Resolve wte_covar : ws.
+Hint Resolve wcs_tyvar : ws.
+Hint Resolve wcs_covar : ws.
+Hint Resolve wcs_tyvari : ws.
+Hint Resolve wcs_covari : ws.
 Hint Resolve wtsub_left : ws.
 Hint Resolve wtsub_right : ws.
 
@@ -498,11 +498,11 @@ Hint Resolve wtsub_right : ws.
 (* Proof. constructor; crush. Qed. *)
 (* Hint Resolve wtSub_wkm_covar : ws. *)
 
-Definition upred (ζγ: Sub Exp) : Sub Exp :=
+Definition upCoSub (ζγ: Sub Exp) : Sub Exp :=
   ((ζγ >=> wkm Exp) · corefl (var 0)).
 
-Lemma wtRed_up_tyvar {Γ Δ ζγd ζγe ζ1 ζ2} (wζ: WtRed Γ Δ ζγd ζγe ζ1 ζ2) :
-  ∀ k, WtRed (Γ ► k) (Δ ► k) (upred ζγd) (upred ζγe) ζ1↑ ζ2↑.
+Lemma wtCoSub_up_tyvar {Γ Δ ζγ ζγi ζ1 ζ2} (wζ: WtCoSub Γ Δ ζγ ζγi ζ1 ζ2) :
+  ∀ k, WtCoSub (Γ ► k) (Δ ► k) (upCoSub ζγ) (upCoSub ζγi) ζ1↑ ζ2↑.
 Proof.
   rewrite ?up_def.
   constructor; intros.
@@ -523,81 +523,85 @@ Proof.
   - rewrite <- ?up_def; crush.
   - rewrite <- ?up_def; crush.
 Qed.
-Hint Resolve wtRed_up_tyvar : ws.
+Hint Resolve wtCoSub_up_tyvar : ws.
 
-Fixpoint apRed (ζγd ζγe ζ1 ζ2: Sub Exp) (τ: Exp) {struct τ} : Exp :=
+Fixpoint apCoSub (ζγ ζγi ζ1 ζ2: Sub Exp) (τ: Exp) {struct τ} : Exp :=
   match τ with
-    | var α              =>  ζγd α
-    | τabs k τ           =>  coτabs k (apRed (upred ζγd) (upred ζγe) ζ1↑ ζ2↑ τ)
-    | τapp τ1 τ2         =>  coτapp (apRed ζγd ζγe ζ1 ζ2 τ1) (apRed ζγd ζγe ζ1 ζ2 τ2)
-    | arr  τ1 τ2         =>  coarr  (apRed ζγd ζγe ζ1 ζ2 τ1) (apRed ζγd ζγe ζ1 ζ2 τ2)
-    | arrτ k τ           =>  coarrτ k (apRed (upred ζγd) (upred ζγe) ζ1↑ ζ2↑ τ)
-    | arrγ τ1 τ2 k τ3    =>  coarrγ (apRed ζγd ζγe ζ1 ζ2 τ1) (apRed ζγd ζγe ζ1 ζ2 τ2) k (apRed ζγd ζγe ζ1 ζ2 τ3)
-    | coτabs k γ         =>  coτabs k (apRed (upred ζγd) (upred ζγe) ζ1↑ ζ2↑ γ)
-    | coτapp γ1 γ2       =>  coτapp (apRed ζγd ζγe ζ1 ζ2 γ1) (apRed ζγd ζγe ζ1 ζ2 γ2)
-    | coarr  γ1 γ2       =>  coarr  (apRed ζγd ζγe ζ1 ζ2 γ1) (apRed ζγd ζγe ζ1 ζ2 γ2)
-    | coarrτ k γ         =>  coarrτ k (apRed (upred ζγd) (upred ζγe) ζ1↑ ζ2↑ γ)
-    | coarrγ γ1 γ2 k γ3  =>  coarrγ (apRed ζγd ζγe ζ1 ζ2 γ1) (apRed ζγd ζγe ζ1 ζ2 γ2) k (apRed ζγd ζγe ζ1 ζ2 γ3)
-    | coinvarr₁ γ        =>  coinvarr₁ (apRed ζγd ζγe ζ1 ζ2 γ)
-    | coinvarr₂ γ        =>  coinvarr₂ (apRed ζγd ζγe ζ1 ζ2 γ)
-    | coinvarrτ γ1 γ2    =>  coinvarrτ (apRed ζγd ζγe ζ1 ζ2 γ1) (apRed ζγd ζγe ζ1 ζ2 γ2)
-    | coinvarrγ₁ γ       =>  coinvarrγ₁ (apRed ζγd ζγe ζ1 ζ2 γ)
-    | coinvarrγ₂ γ       =>  coinvarrγ₂ (apRed ζγd ζγe ζ1 ζ2 γ)
-    | coinvarrγ₃ γ       =>  coinvarrγ₃ (apRed ζγd ζγe ζ1 ζ2 γ)
-    | cobeta γ1 γ2       =>  cobeta (apRed (upred ζγd) (upred ζγe) ζ1↑ ζ2↑ γ1) (apRed ζγd ζγe ζ1 ζ2 γ2)
-    | corefl τ           =>  apRed ζγd ζγe ζ1 ζ2 τ
-    | cosym γ            =>  cosym (apRedSym ζγd ζγe ζ1 ζ2 γ)
-    | cotrans γ1 γ2      =>  cotrans (apRed ζγd ζγe ζ1 ζ2 γ1) γ2[ζ2]
+    | var α              =>  ζγ α
+    | τabs k τ           =>  coτabs k (apCoSub (upCoSub ζγ) (upCoSub ζγi) ζ1↑ ζ2↑ τ)
+    | τapp τ1 τ2         =>  coτapp (apCoSub ζγ ζγi ζ1 ζ2 τ1) (apCoSub ζγ ζγi ζ1 ζ2 τ2)
+    | arr  τ1 τ2         =>  coarr  (apCoSub ζγ ζγi ζ1 ζ2 τ1) (apCoSub ζγ ζγi ζ1 ζ2 τ2)
+    | arrτ k τ           =>  coarrτ k (apCoSub (upCoSub ζγ) (upCoSub ζγi) ζ1↑ ζ2↑ τ)
+    | arrγ τ1 τ2 k τ3    =>  coarrγ (apCoSub ζγ ζγi ζ1 ζ2 τ1) (apCoSub ζγ ζγi ζ1 ζ2 τ2) k (apCoSub ζγ ζγi ζ1 ζ2 τ3)
+    | coτabs k γ         =>  coτabs k (apCoSub (upCoSub ζγ) (upCoSub ζγi) ζ1↑ ζ2↑ γ)
+    | coτapp γ1 γ2       =>  coτapp (apCoSub ζγ ζγi ζ1 ζ2 γ1) (apCoSub ζγ ζγi ζ1 ζ2 γ2)
+    | coarr  γ1 γ2       =>  coarr  (apCoSub ζγ ζγi ζ1 ζ2 γ1) (apCoSub ζγ ζγi ζ1 ζ2 γ2)
+    | coarrτ k γ         =>  coarrτ k (apCoSub (upCoSub ζγ) (upCoSub ζγi) ζ1↑ ζ2↑ γ)
+    | coarrγ γ1 γ2 k γ3  =>  coarrγ (apCoSub ζγ ζγi ζ1 ζ2 γ1) (apCoSub ζγ ζγi ζ1 ζ2 γ2) k (apCoSub ζγ ζγi ζ1 ζ2 γ3)
+    | coinvarr₁ γ        =>  coinvarr₁ (apCoSub ζγ ζγi ζ1 ζ2 γ)
+    | coinvarr₂ γ        =>  coinvarr₂ (apCoSub ζγ ζγi ζ1 ζ2 γ)
+    | coinvarrτ γ1 γ2    =>  coinvarrτ (apCoSub ζγ ζγi ζ1 ζ2 γ1) (apCoSub ζγ ζγi ζ1 ζ2 γ2)
+    | coinvarrγ₁ γ       =>  coinvarrγ₁ (apCoSub ζγ ζγi ζ1 ζ2 γ)
+    | coinvarrγ₂ γ       =>  coinvarrγ₂ (apCoSub ζγ ζγi ζ1 ζ2 γ)
+    | coinvarrγ₃ γ       =>  coinvarrγ₃ (apCoSub ζγ ζγi ζ1 ζ2 γ)
+    | cobeta γ1 γ2       =>  cobeta (apCoSub (upCoSub ζγ) (upCoSub ζγi) ζ1↑ ζ2↑ γ1) (apCoSub ζγ ζγi ζ1 ζ2 γ2)
+    | corefl τ           =>  apCoSub ζγ ζγi ζ1 ζ2 τ
+    | cosym γ            =>  cosym (apCoSubSym ζγ ζγi ζ1 ζ2 γ)
+    | cotrans γ1 γ2      =>  cotrans (apCoSub ζγ ζγi ζ1 ζ2 γ1) γ2[ζ2]
     | _ => var 0
   end
-with apRedSym (ζγd ζγe ζ1 ζ2: Sub Exp) (τ: Exp) {struct τ} : Exp :=
+with apCoSubSym (ζγ ζγi ζ1 ζ2: Sub Exp) (τ: Exp) {struct τ} : Exp :=
   match τ with
-    | var α              =>  ζγe α
-    | τabs k τ           =>  coτabs k (apRedSym (upred ζγd) (upred ζγe) ζ1↑ ζ2↑ τ)
-    | τapp τ1 τ2         =>  coτapp (apRedSym ζγd ζγe ζ1 ζ2 τ1) (apRedSym ζγd ζγe ζ1 ζ2 τ2)
-    | arr  τ1 τ2         =>  coarr  (apRedSym ζγd ζγe ζ1 ζ2 τ1) (apRedSym ζγd ζγe ζ1 ζ2 τ2)
-    | arrτ k τ           =>  coarrτ k (apRedSym (upred ζγd) (upred ζγe) ζ1↑ ζ2↑ τ)
-    | arrγ τ1 τ2 k τ3    =>  coarrγ (apRedSym ζγd ζγe ζ1 ζ2 τ1) (apRedSym ζγd ζγe ζ1 ζ2 τ2) k (apRedSym ζγd ζγe ζ1 ζ2 τ3)
-    | coτabs k γ         =>  coτabs k (apRedSym (upred ζγd) (upred ζγe) ζ1↑ ζ2↑ γ)
-    | coτapp γ1 γ2       =>  coτapp (apRedSym ζγd ζγe ζ1 ζ2 γ1) (apRedSym ζγd ζγe ζ1 ζ2 γ2)
-    | coarr  γ1 γ2       =>  coarr  (apRedSym ζγd ζγe ζ1 ζ2 γ1) (apRedSym ζγd ζγe ζ1 ζ2 γ2)
-    | coarrτ k γ         =>  coarrτ k (apRedSym (upred ζγd) (upred ζγe) ζ1↑ ζ2↑ γ)
-    | coarrγ γ1 γ2 k γ3  =>  coarrγ (apRedSym ζγd ζγe ζ1 ζ2 γ1) (apRedSym ζγd ζγe ζ1 ζ2 γ2) k (apRedSym ζγd ζγe ζ1 ζ2 γ3)
-    | coinvarr₁ γ        =>  coinvarr₁ (apRedSym ζγd ζγe ζ1 ζ2 γ)
-    | coinvarr₂ γ        =>  coinvarr₂ (apRedSym ζγd ζγe ζ1 ζ2 γ)
-    | coinvarrτ γ1 γ2    =>  coinvarrτ (apRedSym ζγd ζγe ζ1 ζ2 γ1) (apRedSym ζγd ζγe ζ1 ζ2 γ2)
-    | coinvarrγ₁ γ       =>  coinvarrγ₁ (apRedSym ζγd ζγe ζ1 ζ2 γ)
-    | coinvarrγ₂ γ       =>  coinvarrγ₂ (apRedSym ζγd ζγe ζ1 ζ2 γ)
-    | coinvarrγ₃ γ       =>  coinvarrγ₃ (apRedSym ζγd ζγe ζ1 ζ2 γ)
-    | cobeta γ1 γ2       =>  cobeta (apRedSym (upred ζγd) (upred ζγe) ζ1↑ ζ2↑ γ1) (apRedSym ζγd ζγe ζ1 ζ2 γ2)
-    | corefl τ           =>  apRedSym ζγd ζγe ζ1 ζ2 τ
-    | cosym γ            =>  cosym (apRed ζγd ζγe ζ1 ζ2 γ)
-    | cotrans γ1 γ2      =>  cotrans γ1[ζ2] (apRedSym ζγd ζγe ζ1 ζ2 γ2)
+    | var α              =>  ζγi α
+    | τabs k τ           =>  coτabs k (apCoSubSym (upCoSub ζγ) (upCoSub ζγi) ζ1↑ ζ2↑ τ)
+    | τapp τ1 τ2         =>  coτapp (apCoSubSym ζγ ζγi ζ1 ζ2 τ1) (apCoSubSym ζγ ζγi ζ1 ζ2 τ2)
+    | arr  τ1 τ2         =>  coarr  (apCoSubSym ζγ ζγi ζ1 ζ2 τ1) (apCoSubSym ζγ ζγi ζ1 ζ2 τ2)
+    | arrτ k τ           =>  coarrτ k (apCoSubSym (upCoSub ζγ) (upCoSub ζγi) ζ1↑ ζ2↑ τ)
+    | arrγ τ1 τ2 k τ3    =>  coarrγ (apCoSubSym ζγ ζγi ζ1 ζ2 τ1) (apCoSubSym ζγ ζγi ζ1 ζ2 τ2) k (apCoSubSym ζγ ζγi ζ1 ζ2 τ3)
+    | coτabs k γ         =>  coτabs k (apCoSubSym (upCoSub ζγ) (upCoSub ζγi) ζ1↑ ζ2↑ γ)
+    | coτapp γ1 γ2       =>  coτapp (apCoSubSym ζγ ζγi ζ1 ζ2 γ1) (apCoSubSym ζγ ζγi ζ1 ζ2 γ2)
+    | coarr  γ1 γ2       =>  coarr  (apCoSubSym ζγ ζγi ζ1 ζ2 γ1) (apCoSubSym ζγ ζγi ζ1 ζ2 γ2)
+    | coarrτ k γ         =>  coarrτ k (apCoSubSym (upCoSub ζγ) (upCoSub ζγi) ζ1↑ ζ2↑ γ)
+    | coarrγ γ1 γ2 k γ3  =>  coarrγ (apCoSubSym ζγ ζγi ζ1 ζ2 γ1) (apCoSubSym ζγ ζγi ζ1 ζ2 γ2) k (apCoSubSym ζγ ζγi ζ1 ζ2 γ3)
+    | coinvarr₁ γ        =>  coinvarr₁ (apCoSubSym ζγ ζγi ζ1 ζ2 γ)
+    | coinvarr₂ γ        =>  coinvarr₂ (apCoSubSym ζγ ζγi ζ1 ζ2 γ)
+    | coinvarrτ γ1 γ2    =>  coinvarrτ (apCoSubSym ζγ ζγi ζ1 ζ2 γ1) (apCoSubSym ζγ ζγi ζ1 ζ2 γ2)
+    | coinvarrγ₁ γ       =>  coinvarrγ₁ (apCoSubSym ζγ ζγi ζ1 ζ2 γ)
+    | coinvarrγ₂ γ       =>  coinvarrγ₂ (apCoSubSym ζγ ζγi ζ1 ζ2 γ)
+    | coinvarrγ₃ γ       =>  coinvarrγ₃ (apCoSubSym ζγ ζγi ζ1 ζ2 γ)
+    | cobeta γ1 γ2       =>  cobeta (apCoSubSym (upCoSub ζγ) (upCoSub ζγi) ζ1↑ ζ2↑ γ1) (apCoSubSym ζγ ζγi ζ1 ζ2 γ2)
+    | corefl τ           =>  apCoSubSym ζγ ζγi ζ1 ζ2 τ
+    | cosym γ            =>  cosym (apCoSub ζγ ζγi ζ1 ζ2 γ)
+    | cotrans γ1 γ2      =>  cotrans γ1[ζ2] (apCoSubSym ζγ ζγi ζ1 ζ2 γ2)
     | _ => var 0
   end.
 
-Lemma ty_red {Γ τ k} (wτ: ⟨ Γ ⊢ τ ∷ k ⟩) :
-  ∀ Δ ζγd ζγe ζ1 ζ2,
-    WtRed Γ Δ ζγd ζγe ζ1 ζ2 →
-    ⟨ Δ ⊢ apRed ζγd ζγe ζ1 ζ2 τ : τ[ζ1] ~ τ[ζ2] ∷ k ⟩
-with ty_redsym {Γ τ k} (wτ: ⟨ Γ ⊢ τ ∷ k ⟩) :
-  ∀ Δ ζγd ζγe ζ1 ζ2,
-    WtRed Γ Δ ζγd ζγe ζ1 ζ2 →
-    ⟨ Δ ⊢ apRedSym ζγd ζγe ζ1 ζ2 τ : τ[ζ2] ~ τ[ζ1] ∷ k ⟩.
+Lemma ty_cosub {Γ τ k} (wτ: ⟨ Γ ⊢ τ ∷ k ⟩) :
+  ∀ Δ ζγ ζγi ζ1 ζ2,
+    WtCoSub Γ Δ ζγ ζγi ζ1 ζ2 →
+    ⟨ Δ ⊢ apCoSub ζγ ζγi ζ1 ζ2 τ : τ[ζ1] ~ τ[ζ2] ∷ k ⟩
+with ty_cosubsym {Γ τ k} (wτ: ⟨ Γ ⊢ τ ∷ k ⟩) :
+  ∀ Δ ζγ ζγi ζ1 ζ2,
+    WtCoSub Γ Δ ζγ ζγi ζ1 ζ2 →
+    ⟨ Δ ⊢ apCoSubSym ζγ ζγi ζ1 ζ2 τ : τ[ζ2] ~ τ[ζ1] ∷ k ⟩.
 Proof.
   - induction wτ; crush.
   - induction wτ; crush.
 Qed.
-Hint Resolve ty_red : ws.
-Hint Resolve ty_redsym : ws.
+Hint Resolve ty_cosub : ws.
+Hint Resolve ty_cosubsym : ws.
 
-Lemma co_red {Γ γ τ1 τ2 k} (wγ: ⟨ Γ ⊢ γ : τ1 ~ τ2 ∷ k ⟩) :
-  ∀ Δ ζγd ζγe ζ1 ζ2, WtRed Γ Δ ζγd ζγe ζ1 ζ2 → ⟨ Δ ⊢ apRed ζγd ζγe ζ1 ζ2 γ : τ1[ζ1] ~ τ2[ζ2] ∷ k ⟩
-with co_redsym {Γ γ τ1 τ2 k} (wγ: ⟨ Γ ⊢ γ : τ1 ~ τ2 ∷ k ⟩) :
-  ∀ Δ ζγd ζγe ζ1 ζ2, WtRed Γ Δ ζγd ζγe ζ1 ζ2 → ⟨ Δ ⊢ apRedSym ζγd ζγe ζ1 ζ2 γ : τ1[ζ2] ~ τ2[ζ1] ∷ k ⟩.
+Lemma co_cosub {Γ γ τ1 τ2 k} (wγ: ⟨ Γ ⊢ γ : τ1 ~ τ2 ∷ k ⟩) :
+  ∀ Δ ζγ ζγi ζ1 ζ2,
+    WtCoSub Γ Δ ζγ ζγi ζ1 ζ2 →
+    ⟨ Δ ⊢ apCoSub ζγ ζγi ζ1 ζ2 γ : τ1[ζ1] ~ τ2[ζ2] ∷ k ⟩
+with co_cosubsym {Γ γ τ1 τ2 k} (wγ: ⟨ Γ ⊢ γ : τ1 ~ τ2 ∷ k ⟩) :
+  ∀ Δ ζγ ζγi ζ1 ζ2,
+    WtCoSub Γ Δ ζγ ζγi ζ1 ζ2 →
+    ⟨ Δ ⊢ apCoSubSym ζγ ζγi ζ1 ζ2 γ : τ1[ζ2] ~ τ2[ζ1] ∷ k ⟩.
 Proof.
   - induction wγ; crush.
   - induction wγ; crush.
 Qed.
-Hint Resolve co_red : ws.
-Hint Resolve co_redsym : ws.
+Hint Resolve co_cosub : ws.
+Hint Resolve co_cosubsym : ws.
